Leansubst.lean
@@ -1,1 +1,3 @@
+import Leansubst.Defs
+
 def hello := "world"
