Leansubst/Defs.lean
@@ -1,0 +1,159 @@
+import Std.Data.Nat.Basic
+import Std.Tactic.Basic
+
+namespace Leansubst
+
+/-! First we define expressions without explicit substitutions and "metavariables".
+    They are also a semantic model for more complex expressions (so-called "de Bruijn algebra"). -/
+
+/-- Abstract syntax tree using de Bruijn indices. -/
+inductive Expr (σ : Type) where
+  | var    : Nat →               Expr σ -- Variable in de Bruijn index.
+  | binder : Expr σ →            Expr σ -- Binder presence.
+  | node   : σ → List (Expr σ) → Expr σ -- Tree node.
+-- Nested inductive types (e.g. the `List Expr` here) are a special case of mutual inductive types.
+
+/-- Renamings. -/
+inductive Renaming where
+  | shift : Nat →            Renaming -- Shift overflow variables up.
+  | cons  : Nat → Renaming → Renaming -- Prepend to sequence.
+
+namespace Renaming
+
+/-- The identity renaming. -/
+def id : Renaming :=
+  shift 0
+
+/-- Evaluate renaming at a given index. -/
+def get : Renaming → Nat → Nat
+  | shift n,  i     => i + n
+  | cons h _, 0     => h
+  | cons _ t, i + 1 => get t i
+
+/-- Composition of renamings. -/
+def comp : Renaming → Renaming → Renaming
+  | shift n,       shift m  => shift (n + m)
+  | shift 0,       cons h t => cons h t
+  | shift (n + 1), cons _ t => comp (shift n) t
+  | cons h t,      r        => cons (r.get h) (comp t r)
+
+/-- Applies a renaming on a term. -/
+def apply {σ} : Renaming → Expr σ → Expr σ
+  | r, .var i     => .var $ r.get i
+  | r, .binder e  => .binder $ apply (cons 0 (comp r (shift 1))) e
+  | r, .node n es => .node n $ applies r es
+where applies {σ} : Renaming → List (Expr σ) → List (Expr σ)
+  | _, []      => []
+  | r, e :: es => apply r e :: applies r es
+termination_by
+  apply _ e    => sizeOf e
+  applies _ es => sizeOf es
+
+end Renaming
+
+/-- Substitutions. -/
+inductive Subst (σ : Type) where
+  | shift : Nat →              Subst σ -- Shift overflow variables up.
+  | cons  : Expr σ → Subst σ → Subst σ -- Prepend to sequence.
+
+namespace Subst
+
+def fromRenaming (σ) : Renaming → Subst σ
+  | .shift n  => shift n
+  | .cons h t => cons (.var h) (fromRenaming σ t)
+
+instance {σ} : Coe Renaming (Subst σ) :=
+  ⟨fromRenaming σ⟩
+
+/-- The identity substitution. -/
+def id (σ) : Subst σ :=
+  shift 0
+
+/-- Evaluate substitution at a given index. -/
+def get {σ} : Subst σ → Nat → Expr σ
+  | shift n,  i     => .var (i + n)
+  | cons h _, 0     => h
+  | cons _ t, i + 1 => get t i
+
+/-- Composition of substitution and renaming. -/
+def compr {σ} : Subst σ → Renaming → Subst σ
+  | shift n,  r => Renaming.comp (.shift n) r
+  | cons h t, r => cons (r.apply h) (compr t r)
+
+/-- Applies a substitution on a term. -/
+def apply {σ} : Subst σ → Expr σ → Expr σ
+  | shift n,     .var i       => .var (i + n)
+  | cons h _,    .var 0       => h
+  | cons _ t,    .var (i + 1) => apply t (.var i)
+  | s,           .binder e    => .binder (apply (cons (.var 0) (compr s (.shift 1))) e)
+  | s,           .node n es   => .node n (applies s es)
+where applies {σ} : Subst σ → List (Expr σ) → List (Expr σ)
+  | _, []      => []
+  | s, e :: es => apply s e :: applies s es
+termination_by
+  apply s e    => (sizeOf e, sizeOf s)
+  applies s es => (sizeOf es, sizeOf s)
+
+/-- Composition of substitutions. -/
+def comp {σ} : Subst σ → Subst σ → Subst σ
+  | shift n,       shift m  => shift (n + m)
+  | shift 0,       cons h t => cons h t
+  | shift (n + 1), cons _ t => comp (shift n) t
+  | cons h t,      r        => cons (r.apply h) (comp t r)
+
+end Subst
+
+/-! Now define expressions **with** explicit substitutions and "metavariables". -/
+
+mutual
+/-- Explicit substitutions using de Bruijn indices. -/
+inductive ES (σ : Type) where
+  | subst  : ES σ → SE σ →     ES σ -- Substitution application.
+  | zero   :                   ES σ -- Variable with de Bruijn index 0.
+  | binder : ES σ →            ES σ -- Binder presence.
+  | node   : σ → List (ES σ) → ES σ -- Tree node.
+  | mvar   : Nat →             ES σ -- Expression "metavariable".
+
+/-- Substition expressions using de Bruijn indices. -/
+inductive SE (σ : Type) where
+  | shift :               SE σ -- Shift overflow variables up by 1.
+  | cons  : ES σ → SE σ → SE σ -- Prepend to sequence.
+  | comp  : SE σ → SE σ → SE σ -- Chaining (composition) of substitutions.
+  | mvar  : Nat →         SE σ -- Substitution "metavariable".
+end
+
+/-- Variable with arbitrary de Bruijn index. -/
+def ES.var (σ) : Nat → ES σ
+  | 0     => zero
+  | i + 1 => subst (ES.var σ i) .shift
+
+/-- The identity substitution. -/
+def SE.id (σ) : SE σ :=
+  cons .zero shift
+
+/-- Metavariable assignment. -/
+structure Assignment (σ : Type) where
+  es : Nat → Expr σ
+  se : Nat → Subst σ
+
+mutual
+/-- Assign metavariables. -/
+def ES.assign {σ} : Assignment σ → ES σ → Expr σ
+  | a, .subst e s => Subst.apply (SE.assign a s) (ES.assign a e)
+  | _, .zero      => .var 0
+  | a, .binder e  => .binder (ES.assign a e)
+  | a, .node n es => .node n (ES.assigns a es)
+  | a, .mvar i    => a.es i
+where ES.assigns {σ} : Assignment σ → List (ES σ) → List (Expr σ)
+  | _, []         => []
+  | a, e :: es    => ES.assign a e :: ES.assigns a es
+
+/-- Assign metavariables. -/
+def SE.assign {σ} : Assignment σ → SE σ → Subst σ
+  | _, .shift     => .shift 1
+  | a, .cons h t  => .cons (ES.assign a h) (SE.assign a t)
+  | a, .comp s t  => .comp (SE.assign a s) (SE.assign a t)
+  | a, .mvar i    => a.se i
+end
+
+end Leansubst
